Update windows.

src/coq/lang.v
@@ -1,49 +1,59 @@
 Require Import ml.
 Require Import String.
 Require Import List.
+Require Import Classical.
 
 Module Lang <: Formulas.
 
-  Inductive Var : Type := var : string -> string -> Var.
+(*  Inductive Var : Type := var : string -> string -> Var. *)
   Open Scope string_scope.
 
   (* syntax *)
+  Inductive ExpVar : Type := exp_v : string -> ExpVar.
   Inductive Exp : Type := 
-  | exp_var : Var -> Exp
+  | exp_var : ExpVar -> Exp
   | id : string -> Exp
   | val : nat -> Exp
   | plus : Exp -> Exp -> Exp.
+  
 
-  Eval compute in (exp_var (var "a" "exp")).
-  Eval compute in (plus (id "a") (exp_var (var "a" "exp"))).
+  Eval compute in (exp_var (exp_v "a")).
+  Eval compute in (plus (id "a") (exp_var (exp_v "a"))).
   Eval compute in (plus (id "a") (val 4)).
 
+  Inductive StmtVar : Type := stmt_v : string -> StmtVar.
   Inductive Stmt : Type :=
+  | stmt_var : StmtVar -> Stmt 
   | assign : string -> Exp -> Stmt
-  | seq : list Stmt -> Stmt
-  | stmt_var : Var -> Stmt.
+  | seq : list Stmt -> Stmt.
 
   Eval compute in (assign "a" (val 10)).
   Eval compute in (assign "a" (plus (id "a") (val 10))).
   Eval compute in 
       assign "a" (plus (id "a") (val 10)) :: (assign "a" (val 10)) :: nil.
-                   
-  
 
   (* configuration *)
-  Inductive MapItem := item : string -> Exp -> MapItem.
+  Inductive MapItemVar : Type := mi_v : string -> MapItemVar.
+  Inductive MapItem := 
+  | mapitem_var : MapItemVar -> MapItem
+  | item : string -> Exp -> MapItem.
+
+  Inductive CfgVar : Type := cfg_v : string -> CfgVar.
   Inductive Cfg := 
   | cfg : Stmt -> list MapItem -> Cfg
-  | cfg_var : Var -> Cfg.
+  | cfg_var : CfgVar -> Cfg.
 
   Notation "A |-> B" := (item A B) (at level 100).
   Eval compute in (cfg 
                      (assign "a" (plus (id "a") (val 10))) 
-                     (("a" |-> (exp_var (var "A" "exp"))) :: nil)).
+                     (("a" |-> (exp_var (exp_v "A"))) :: nil)).
 
-
-
-
+  (* Var *)
+  Inductive Var : Type :=
+  | var_exp : ExpVar -> Var
+  | var_stmt : StmtVar -> Var
+  | var_mapitem : MapItemVar -> Var 
+  | var_cfg : CfgVar -> Var.
 
   
   (* model and state *)
@@ -67,14 +77,31 @@ Module Lang <: Formulas.
 
 
   (* var equality *)
+  Definition var_eq_exp (X Y : ExpVar) : bool := 
+    match X, Y with 
+      | exp_v x, exp_v y => if string_dec x y then true else false
+    end.
+  Definition var_eq_stmt (X Y : StmtVar) : bool := 
+    match X, Y with 
+      | stmt_v x, stmt_v y => if string_dec x y then true else false
+    end.
+  Definition var_eq_mapitem (X Y : MapItemVar) : bool := 
+    match X, Y with 
+      | mi_v x, mi_v y => if string_dec x y then true else false
+    end.
+  Definition var_eq_cfg (X Y : CfgVar) : bool := 
+    match X, Y with 
+      | cfg_v x, cfg_v y => if string_dec x y then true else false
+    end.
+
+
   Definition var_eq (X Y : Var) : bool :=
     match X, Y with
-      | var x xsort, var y ysort =>
-                     if (string_dec x y) 
-                     then if (string_dec xsort ysort)
-                          then true
-                          else false
-                     else false
+      | var_exp x, var_exp y => var_eq_exp x y
+      | var_stmt x, var_stmt y => var_eq_stmt x y
+      | var_mapitem x, var_mapitem y => var_eq_mapitem x y
+      | var_cfg x, var_cfg y => var_eq_cfg x y
+      | _, _ => false
     end.
 
   Lemma var_eq_true : 
@@ -82,51 +109,61 @@ Module Lang <: Formulas.
   Proof.
     intros a b.
     split; intros H.
-    - unfold var_eq in H.
-      case_eq a; intros aname asort Ha.
-      subst a.
-      case_eq b; intros bname bsort Hb.
-      subst b.
-      case_eq (string_dec aname bname); intros e He; subst; rewrite He in *.
-      + case_eq (string_dec asort bsort); intros e' He'; subst; rewrite He' in *.
-        * trivial.
-        * inversion H.
-      + inversion H.
-    - rewrite H.
+    - case_eq a; intros v Hv; case_eq b; intros v' Hv'; unfold var_eq in H; subst; try inversion H.
+      + unfold var_eq_exp in H.
+        case_eq v; intros v0 Hv0; subst.
+        case_eq v'; intros v0' Hv0'; subst.
+        case_eq (string_dec v0 v0'); intros; subst; trivial.
+        rewrite H0 in H.
+        inversion H.
+      + unfold var_eq_stmt in H.
+        case_eq v; intros v0 Hv0; subst.
+        case_eq v'; intros v0' Hv0'; subst.
+        case_eq (string_dec v0 v0'); intros; subst; trivial.
+        rewrite H0 in H.
+        inversion H.
+      + unfold var_eq_mapitem in H.
+        case_eq v; intros v0 Hv0; subst.
+        case_eq v'; intros v0' Hv0'; subst.
+        case_eq (string_dec v0 v0'); intros; subst; trivial.
+        rewrite H0 in H.
+        inversion H.
+      + unfold var_eq_cfg in H.
+        case_eq v; intros v0 Hv0; subst.
+        case_eq v'; intros v0' Hv0'; subst.
+        case_eq (string_dec v0 v0'); intros; subst; trivial.
+        rewrite H0 in H.
+        inversion H.
+    - subst.
       unfold var_eq.
-      case_eq b; intros bname bsort Hb.
-      case_eq (string_dec bname bname); intros H' H''.
-      + case_eq (string_dec bsort bsort); intros H0 H1; trivial.
-        contradict H1; unfold not in *; intros; apply H0; trivial.
-      + contradict H''; unfold not in *; intros; apply H'; trivial.
+      case_eq b; intros e He.
+      + unfold var_eq_exp; case_eq e; intros s Hs; case_eq (string_dec s s); intros; trivial.
+        contradiction n; trivial.
+      + unfold var_eq_stmt; case_eq e; intros s Hs; case_eq (string_dec s s); intros; trivial.
+        contradiction n; trivial.
+      + unfold var_eq_mapitem; case_eq e; intros s Hs; case_eq (string_dec s s); intros; trivial.
+        contradiction n; trivial.
+      + unfold var_eq_cfg; case_eq e; intros s Hs; case_eq (string_dec s s); intros; trivial.
+        contradiction n; trivial.
   Qed.
 
   Lemma var_eq_false:
     forall a b, var_eq a b = false <-> a <> b.
   Proof.
-    intros a b; split; intros H.
-    - unfold var_eq in *.
-      case_eq a; intros aname asort Ha.
-      case_eq b; intros bname bsort Hb.
-      rewrite Ha, Hb in H.
-      case_eq (string_dec aname bname); intros e He; subst; rewrite He in *.
-      + case_eq (string_dec asort bsort); intros e He'; subst; rewrite He' in *.
-        * inversion H.
-        * unfold not in *; intros; apply e.
-          inversion H0; trivial.
-      + unfold not in *; intros; apply e.
-        inversion H0; trivial.
-    - case_eq a; intros aname asort Ha.
-      case_eq b; intros bname bsort Hb.
-      subst.
-      unfold var_eq.
-      case_eq (string_dec aname bname); intros e He; subst; trivial.
-      case_eq (string_dec asort bsort); intros e He'; subst; trivial.
-      contradict H.
-      apply var_eq_true.
-      simpl.
-      rewrite He, He'; trivial.
-  Qed.
+    intros a b.
+    split; intros H.
+    - unfold not.
+      intros H'.
+      apply var_eq_true in H'.
+      rewrite H in H'.
+      inversion H'.
+    - assert (H' : var_eq a b = false \/ ~ var_eq a b = false ).
+      apply classic.
+      destruct H' as [H' | H']; trivial.
+      case_eq (var_eq a b); intros Hv; trivial.
+      rewrite var_eq_true in Hv.
+      contradict H; trivial.
+ Qed.
 
   Lemma var_eq_refl : 
     forall x, var_eq x x = true.
